Model/StatefulDataflow.v
@@ -1,104 +1,115 @@
-(* TODO refactor, think about modules/parameters (probably there is a better way to do it) *)
 From Coq Require Import String List Vector.
 From Model Require Import Streaming.
 Import ListNotations.
+Import StreamingNotations.
 
-Module Type StatefulDataflowTypes.
-  Parameter eventValueType: Type.
-  Parameter stateValueType: Type.
-End StatefulDataflowTypes.
+Section StatefulDataflow.
 
-Module StatefulDataflowParameters (T: StatefulDataflowTypes) <: Parameters.
-  Import T.
-  Implicit Types (w: eventValueType).
-  Implicit Types (v: stateValueType).
-  Implicit Types (n e: nat).
-  Implicit Types (s o r t: string).
+Class SDParameters: Type :=
+  { countOfProcessors: nat
+  ; StateValue: Type
+  ; EventValue: Type }.
+Context { sdParametersContext: SDParameters }.
 
-  Inductive ProcessorType := lltask (f: stateValueType * eventValueType -> stateValueType * list eventValueType) (ss: list string) o.
-  Definition Processor := ProcessorType.
+(* Values *)
+Implicit Types (v: StateValue).
+Implicit Types (w: EventValue).
+Implicit Types (W: list EventValue).
 
-  Inductive llstatecase := failed | normal e v.
-  Definition Archive := list stateValueType.
-  Implicit Types (a: Archive).
-  Definition State: Type := Archive * llstatecase.
+(* Epoch Number *)
+Implicit Types (e: nat).
 
-  Inductive lldatacase := event w | border.
-  Definition MessageData: Type := nat * lldatacase.
-  Implicit Types (d: MessageData).
-
-  Inductive Message := message n s d.
-  Definition AuxiliaryData: Type := list Message.
-End StatefulDataflowParameters.
-
-Module StatefulDataflow (C: CountOfProcessors) (T: StatefulDataflowTypes).
-Module SDP := StatefulDataflowParameters T.
-Module StatefulDataflowSystem := Streaming C SDP.
-Export StatefulDataflowSystem.
-Export T.
-
-Implicit Types (v: stateValueType).
-Implicit Types (w: eventValueType).
-Implicit Types (W: list eventValueType).
+(* Processor ID *)
 Implicit Types (p q: Fin.t countOfProcessors).
+
+(* Stream Name *)
 Implicit Types (s o r t: string).
-Implicit Types (n e: nat).
+
+(* Sequence Number or Length of Sequence *)
+Implicit Types (n: nat).
+
+(* Sequence Index *)
 Implicit Types (i j: nat).
+
+(* Processor *)
+Inductive Processor := lltask (f: StateValue * EventValue -> StateValue * list EventValue) (ss: list string) o.
 Implicit Types (pi: Processor).
-Implicit Types (Pi: Processors).
+
+(* State *)
+Inductive llstatecase := failed | normal e v.
+Definition Archive := list StateValue.
+Implicit Types (a: Archive).
+Definition State: Type := Archive * llstatecase.
 Implicit Types (sigma Sigmap: State).
-Implicit Types (Sigma: States).
+
+(* Message Data *)
+Inductive lldatacase := event w | border.
+Definition MessageData: Type := nat * lldatacase.
 Implicit Types (d: MessageData).
-Implicit Types (m: Message).
-Implicit Types (M: Messages).
-Implicit Types (Np: SequenceNumbers).
-Implicit Types (N: AllSequenceNumbers).
-Implicit Types (D: AuxiliaryData).
+
+(* Auxiliary Data *)
+Definition AuxiliaryData := list (nat * string * MessageData).
+
+Instance sParameters: SParameters :=
+  {| SCountOfProcessors := countOfProcessors
+   ; SProcessor     := Processor
+   ; SState         := State
+   ; SMessageData   := MessageData
+   ; SAuxiliaryData := AuxiliaryData |}.
 
 Reserved Notation "pi '||-' sigma '-(' X ')->l' sigma'" (at level 60).
 Inductive lsteps: Processor -> State -> list Action -> State -> Prop :=
 | l_event: forall f ss o a e v s w W' v',
   (v', W') = f(v, w) ->
-  lltask f ss o ||- (a, normal e v) -([`- s (e, event w)] ++ List.map (fun w' => `+ o (e, event w')) W')->l (a, normal e v')
+  lltask f ss o ||- (a, normal e v) -([`- s (e, event w)] ++ List.map (fun w' => `+ o (e, event w')) W' )->l (a, normal e v')
 | l_border: forall f ss o a e v s,
   lltask f ss o ||-
   (a, normal e v)
-  -(List.map (fun s => `- s (e, border)) ss ++ [`+ o (e, border)])->l
+  -(List.map (fun s => `- s (e, border)) ss ++ [produce o (e, border)])->l
   (a++[v], normal (e+1) v)
 where "pi '||-' sigma '-(' X ')->l' sigma'" := (lsteps pi sigma X sigma').
 
-Reserved Notation "pi '||-' sigma1 '-(' X ')->f' sigma2" (at level 60).
+Reserved Notation "pi '||-' sigma '-(' X ')->f' sigma'" (at level 60).
 Inductive fsteps: Processor -> State -> list Action -> State -> Prop :=
 | f_fail: forall pi a sigmal, pi ||- (a, sigmal) -([])->f (a, failed)
 where "pi '||-' sigma '-(' X ')->f' sigma'" := (fsteps pi sigma X sigma').
 
-Definition local pi sigma A sigma': Prop := lsteps pi sigma A sigma' \/ fsteps pi sigma A sigma'.
+Definition local pi sigma X sigma': Prop :=
+  pi ||- sigma -(X)->l sigma' \/
+  pi ||- sigma -(X)->f sigma'.
 Notation "pi ||- sigma -( X )-> sigma'" := (local pi sigma X sigma') (at level 60).
 
-Definition gce (C: Configuration): nat := match C with (Pi, Sigma, N, M, D) =>
+Definition gce (c: Configuration): nat := match c with (Pi, Sigma, N, M, D) =>
   fold_left (fun acc sigma => match sigma with (a, sigmal) => min acc (List.length a) end) 0 Sigma
 end.
 
-Definition out C: Messages := match C with (Pi, Sigma, N, M, D) =>
-  List.filter (fun m => match m with message n s (e, dd) => Nat.leb e (gce C) end) M
+Definition out c: Messages := match c with (Pi, Sigma, N, M, D) =>
+  List.filter (fun m => match m with (n, s, (e, dd)) => Nat.leb e (gce c) end) M
 end.
 
-Definition snapshotOf C: Configuration := match C with (Pi, Sigma, N, M, D) =>
-  (Pi,
-  Sigma,
-  N,
-  List.filter (fun m => match m with message n s (e, dd) => Nat.ltb (gce C) e end) M ++ out C,
-  D)
+Definition onStream s M: Messages :=
+  List.filter (fun m => match m with (n, s', (e, dd)) => String.eqb s' s end) M.
+
+Definition lcs c: Configuration := match c with (Pi, Sigma, N, M, D) =>
+  ( Pi
+  , Vector.map (fun sigma => match sigma with (a, sigmav) =>
+    ( firstn (gce c + 1) a
+    , match (List.nth_error a (gce c)) with None => failed |
+      Some v => normal (gce c + 1) v
+    end) end) Sigma
+  , Vector.map (fun Np => List.map (fun sn => match sn with (s, n) => (s, length (onStream s (out c))) end) Np) N
+  , List.filter (fun m => match m with (n, s, (e, dd)) => Nat.ltb (gce c) e end) D ++ out c
+  , D )
 end.
 
-Reserved Notation "C '=>f' C'" (at level 60).
+Reserved Notation "c '=>f' c'" (at level 60).
 Inductive fSteps: Configuration -> Configuration -> Prop :=
 | f_recover: forall Pi Sigma N M D p a,
   nth Sigma p = (a, failed) ->
-  (Pi, Sigma, N, M, D) =>f snapshotOf (Pi, Sigma, N, M, D)
-where "C '=>f' C'" := (fSteps C C').
+  (Pi, Sigma, N, M, D) =>f lcs (Pi, Sigma, N, M, D)
+where "c '=>f' c'" := (fSteps c c').
 
-Definition F C C': Prop := StreamingAbsP fsteps C C' \/ fSteps C C'.
-Definition L C C': Prop := StreamingAbsP local C C' \/ fSteps C C'.
+Definition F c c': Prop := StreamingAbsP fsteps c c' \/ fSteps c c'.
+Definition L c c': Prop := StreamingAbsP local c c' \/ fSteps c c'.
 
 End StatefulDataflow.
